# Expression of the mixed derivatives of the energy

$$
\newcommand{\E}{\mathcal{E}}
\newcommand{\reals}{\mathbb{R}}
$$

Eq. (@eq-20221227184138) holds for all $\lambda$. Upon successive derivations with respect to $\lambda$, it is found
that, for all $\hat{u} \in U$ and $\lambda \in \reals$

$$
\E_{,uu}[u^\ast(\lambda), \lambda; \dot{u}^\ast(\lambda), \hat{u}] + \E_{,u\lambda}[u^\ast(\lambda), \lambda; \hat{u}] = 0
$$

and

$$
\begin{aligned}[b]
\E_{,uuu}[u^\ast(\lambda), \lambda; \dot{u}^\ast(\lambda), \dot{u}^\ast(\lambda), \hat{u}] + 2\E_{,uu\lambda}[u^\ast(\lambda), \lambda; \dot{u}^\ast(\lambda), \hat{u}] &\\
+ \E_{,u\lambda\lambda}[u^\ast(\lambda), \lambda; \hat{u}] + \E_{,uu}[u^\ast(\lambda), \lambda; \ddot{u}^\ast(\lambda), \hat{u}] &= 0
\end{aligned}
$$

and, at the critical point

$$
\begin{gather}
  \E_2(\dot{u}_0, \bullet) + \E_{,u\lambda}(u_0, \lambda_0; \bullet) = 0,\\
  \E_3(\dot{u}_0, \dot{u}_0, \bullet) + 2\E_{,uu\lambda}(u_0, \lambda_0; \dot{u}_0, \bullet) + \E_{,u\lambda\lambda}(u_0, \lambda_0; \bullet) + \E_2(\ddot{u}_0, \bullet) = 0.
\end{gather}
$$

Combining with Eq. (@eq-20221227184821), the mixed derivatives $\E_{,u\lambda}(u_0, \lambda_0; \bullet)$,
$\E_{,uu\lambda}(u_0, \lambda_0; \bullet, \bullet)$ and $\E_{,u\lambda\lambda}(u_0, \lambda_0; \bullet)$ can be
expressed as functions of $u_0$, $\dot{u}_0$, $\ddot{u}_0$, $\E_2$ and $\E_3$. More generally, it is shown in Appendix
**compléter référence** that the following mixed derivatives can be thus expressed

$$
\E_{,u\lambda}(u_0, \lambda_0; \bullet) = -\E_2(\dot{u}_0, \bullet),
$$

$$
\E_{,uu\lambda}(u_0, \lambda_0; \bullet, \bullet) = -\E_3(\dot{u}_0, \bullet, \bullet) + \dot{\E}_2(\bullet, \bullet),
$$

$$
\E_{,u\lambda\lambda}(u_0, \lambda_0; \bullet) = - \E_2(\ddot{u}_0, \bullet) - 2\dot{\E}_2(\dot{u}_0, \bullet) + \E_3(\dot{u}_0, \dot{u}_0, \bullet),
$$

$$
\E_{,uuu\lambda}(u_0, \lambda_0; \bullet, \bullet, \bullet) = -\E_4(\dot{u}_0, \bullet, \bullet, \bullet) + \dot{\E}_3(\bullet, \bullet, \bullet),
$$

$$
\E_{,uu\lambda\lambda}(u_0, \lambda_0; \bullet, \bullet) = - \E_3(\ddot{u}_0, \bullet, \bullet) + \ddot{\E}_2(\bullet, \bullet) - 2\dot{\E}_3(\dot{u}_0, \bullet, \bullet) + \E_4(\dot{u}_0, \dot{u}_0, \bullet, \bullet),
$$

$$
\begin{aligned}
\E_{,u\lambda\lambda\lambda}(u_0, \lambda_0; \bullet) ={} & -\E_2(\dddot{u}_0, \bullet) + 3\E_3(\dot{u}_0, \ddot{u}_0, \bullet) - \E_4(\dot{u}_0, \dot{u}_0, \dot{u}_0, \bullet) - 3\ddot{\E}_2(\dot{u}_0, \bullet)\\
  &-3\dot{\E}_2(\ddot{u}_0, \bullet)+ 3\dot{\E}_3(\dot{u}_0, \dot{u}_0, \bullet).
\end{aligned}
$$
